rewrote weakestPrecondition semantics a bit more nicely. made it to sound_cmd'

bedrock2/src/bedrock2/WeakestPrecondition.v
@@ -21,27 +21,31 @@ Section WeakestPrecondition.
 
   Section WithMemAndLocals.
     Context (m : mem) (l : locals).
-    Definition expr_body rec (e : Syntax.expr) (post : trace -> word -> Prop) : Prop :=
+    (* conceptually, maybe it doesn't make a great deal of sense to pass in the trace, and we
+       should just rewrite this function so that it's like we're always passing in a trace of nil.
+       it's easier to work with this way, though. *)
+    Definition expr_body rec (t : trace) (e : Syntax.expr) (post : trace -> word -> Prop) : Prop :=
       match e with
       | expr.literal v =>
-        literal v (post nil)
+        literal v (post t)
       | expr.var x =>
-        get l x (post nil)
+        get l x (post t)
       | expr.op op e1 e2 =>
-        rec e1 (fun t1 v1 =>
-        rec e2 (fun t2 v2 =>
-        post (app t2 t1) (interp_binop op v1 v2)))
+        rec t e1 (fun t' v1 =>
+        rec t' e2 (fun t'' v2 =>
+        post t'' (interp_binop op v1 v2)))
       | expr.load s e =>
-        rec e (fun t a =>
-        load s m a (post (cons (read s a) t)))
+        rec t e (fun t' a =>
+        load s m a (post (cons (read s a) t')))
       | expr.inlinetable s tbl e =>
-        rec e (fun t a =>
-        load s (map.of_list_word tbl) a (post t))
+        rec t e (fun t' a =>
+        load s (map.of_list_word tbl) a (post t'))
       | expr.ite c e1 e2 =>
-        rec c (fun t1 b => rec (if word.eqb b (word.of_Z 0) then e2 else e1) (fun t2 v =>
-        post (app t2 t1) v))
+        rec t c (fun t' b =>
+        rec t' (if word.eqb b (word.of_Z 0) then e2 else e1) (fun t'' v =>
+        post t'' v))
     end.
-    Fixpoint expr e := expr_body expr e.
+    Fixpoint expr t e := expr_body expr t e.
   End WithMemAndLocals.
 
    Section WithF.
@@ -57,40 +61,54 @@ Section WeakestPrecondition.
     Fixpoint list_map xs := list_map_body list_map xs.
    End WithF.
 
-  Section WithF2.
-    Context {A B C} (f: A -> (B -> C -> Prop) -> Prop).
-    Definition list_map2_body rec (xs : list A) (post : list B -> list C -> Prop) : Prop :=
+   Section WithF'.
+    Context {A B T} (f: T -> A -> (T -> B -> Prop) -> Prop).
+    Definition list_map'_body rec (acc : T) (xs : list A) (post : T -> list B -> Prop) : Prop :=
       match xs with
-      | nil => post nil nil
+      | nil => post acc nil
       | cons x xs' =>
-        f x (fun y z =>
-        rec xs' (fun ys' zs' =>
-        post (cons y ys') (cons z zs')))
+        f acc x (fun acc' y =>
+        rec acc' xs' (fun acc'' ys' =>
+        post acc'' (cons y ys')))
+      end. Check list_map'_body.
+    Fixpoint list_map' acc xs := list_map'_body list_map' acc xs.
+   End WithF'.
+
+  (*Section WithF2.
+    Context {A B C} (f: C -> A -> (C -> B -> Prop) -> Prop).
+    Definition list_map2_body rec (xs : list A) (acc : C) (post : list B -> C -> Prop) : Prop :=
+      match xs with
+      | nil => post nil acc 
+      | cons x xs' =>
+        f acc x (fun y z =>
+        rec xs' z (fun ys' z' =>
+        post (cons y ys') z'))
       end.
     Fixpoint list_map2 xs := list_map2_body list_map2 xs.
-  End WithF2.
+  End WithF2.*)
   
   Section WithFunctions.
     Context (call : String.string -> trace -> mem -> list word -> (trace -> mem -> list word -> Prop) -> Prop).
-    Definition dexpr m l e v t := expr m l e (fun t' v' => eq t t' /\ eq v v'). Check dexpr.
-    Definition dexprs m l es vs ts := list_map2 (expr m l) es (fun ts' vs' => eq ts ts' /\ eq vs vs'). Check dexprs. Check expr.
+    Definition dexpr m l t e v t' := expr m l t e (fun t'2 v2 => eq t' t'2 /\ eq v v2).
+    Definition dexprs m l t es vs t' := list_map' (expr m l) t es (fun t'2 vs2 => eq t' t'2 /\ eq vs vs2).
+    Goal (forall m l t, dexprs m l t (cons (expr.load access_size.one (expr.literal 5)) nil) = dexprs m l t nil). cbv [dexprs]. simpl. Abort.
     Definition cmd_body (rec:_->_->_->_->_->Prop) (c : cmd) (t : trace) (m : mem) (l : locals)
              (post : trace -> mem -> locals -> Prop) : Prop :=
       (* give value of each pure expression when stating its subproof *)
       match c with
       | cmd.skip => post t m l
       | cmd.set x ev =>
-        exists v tv, dexpr m l ev v tv /\
+        exists v t', dexpr m l t ev v t' /\
         dlet! l := map.put l x v in
-        post (app tv t) m l
+        post t' m l
       | cmd.unset x =>
         dlet! l := map.remove l x in
         post t m l
       | cmd.store sz ea ev =>
-        exists a ta, dexpr m l ea a ta /\
-        exists v tv, dexpr m l ev v tv /\
+        exists a t', dexpr m l t ea a t' /\
+        exists v t'', dexpr m l t' ev v t'' /\
         store sz m a v (fun m =>
-        post (cons (write sz a) (app tv (app ta t))) m l)
+        post (cons (write sz a) t'') m l)
       | cmd.stackalloc x n c =>
         Z.modulo n (bytes_per_word width) = 0 /\
         forall a mStack mCombined,
@@ -101,9 +119,9 @@ Section WeakestPrecondition.
           anybytes a n mStack' /\ map.split mCombined' m' mStack' /\
           post t' m' l')
       | cmd.cond br ct cf =>
-        exists v tv, dexpr m l br v tv /\
-        (word.unsigned v <> 0%Z -> rec ct (cons (branch true) (app tv t)) m l post) /\
-        (word.unsigned v = 0%Z -> rec cf (cons (branch false) (app tv t)) m l post)
+        exists v t', dexpr m l t br v t' /\
+        (word.unsigned v <> 0%Z -> rec ct (cons (branch true) t') m l post) /\
+        (word.unsigned v = 0%Z -> rec cf (cons (branch false) t') m l post)
       | cmd.seq c1 c2 =>
         rec c1 t m l (fun t m l => rec c2 t m l post)
       | cmd.while e c =>
@@ -111,22 +129,22 @@ Section WeakestPrecondition.
         Coq.Init.Wf.well_founded lt /\
         (exists v, inv v t m l) /\
         (forall v t m l, inv v t m l ->
-          exists b tb, dexpr m l e b tb /\
-          (word.unsigned b <> 0%Z -> rec c (cons (branch true) (app tb t)) m l (fun t' m l =>
+          exists b t', dexpr m l t e b t' /\
+          (word.unsigned b <> 0%Z -> rec c (cons (branch true) t') m l (fun t' m l =>
             exists v', inv v' t' m l /\ lt v' v)) /\
-          (word.unsigned b = 0%Z -> post (cons (branch false) (app tb t)) m l))
+            (word.unsigned b = 0%Z -> post (cons (branch false) t') m l))
       | cmd.call binds fname arges =>
-        exists args targs, dexprs m l arges args targs /\ (* (call : String.string -> trace -> mem -> list word -> (trace -> mem -> list word -> Prop) -> Prop) *)
-        call fname (app (List.concat (List.rev targs)) t) m args (fun t m rets =>
+        exists args t', dexprs m l t arges args t' /\ (* (call : String.string -> trace -> mem -> list word -> (trace -> mem -> list word -> Prop) -> Prop) *)
+        call fname t' m args (fun t'' m rets =>
           exists l', map.putmany_of_list_zip binds rets l = Some l' /\
-          post t m l')
+          post t'' m l')
       | cmd.interact binds action arges =>
-        exists args targs, dexprs m l arges args targs /\
+        exists args t', dexprs m l t arges args t' /\
         exists mKeep mGive, map.split m mKeep mGive /\
-        ext_spec (app (List.concat (List.rev targs)) t) mGive action args (fun mReceive rets =>
+        ext_spec t' mGive action args (fun mReceive rets =>
           exists l', map.putmany_of_list_zip binds rets l = Some l' /\
           forall m', map.split m' mKeep mReceive ->
-          post (cons (IOevent ((mGive, action, args), (mReceive, rets))) (app (List.concat (List.rev targs)) t)) m' l')
+          post (cons (IOevent ((mGive, action, args), (mReceive, rets))) t') m' l')
       end.
     Fixpoint cmd c := cmd_body cmd c.
   End WithFunctions.
@@ -147,11 +165,10 @@ Section WeakestPrecondition.
       then func (rec functions) decl t m args post
       else rec functions fname t m args post
     end.
-  Fixpoint call functions := call_body call functions. Check func.
+  Fixpoint call functions := call_body call functions.
 
   Definition program funcs main t m l post : Prop := cmd (call funcs) main t m l post.
 End WeakestPrecondition.
-Check cmd.
 Ltac unfold1_cmd e :=
   lazymatch e with
     @cmd ?width ?BW ?word ?mem ?locals ?ext_spec ?CA ?c ?t ?m ?l ?post =>
